IGrammarSafety.v
@@ -3,149 +3,112 @@ Require Import MyUtils.
 
 Section IGrammarSafety.
 
-Arguments ANode {_ _} _.
-Arguments INode {_ _} _ _ _.
+(* Search Decision. *)
 
-Arguments HPatt {_}.
-Arguments IPatt {_} _ _ _.
+Create HintDb IGrammar.
+Hint Resolve CPrio1 : IGrammar.
+Hint Resolve CPrio2 : IGrammar.
+Hint Resolve CLeft : IGrammar.
+Hint Resolve CRight : IGrammar.
+Hint Resolve HMatch : IGrammar.
+Hint Resolve IMatch : IGrammar.
 
-Arguments prio {_} _ _ _.
-Arguments left_a {_} _ _ _.
-Arguments right_a {_} _ _ _.
-
-(* Existential Lemmas *)
-
-Lemma dec_conflict_pattern {O} (pr : drules O) `{drules_dec pr} (q : tree_pattern O) :
-  Decision (conflict_pattern pr q).
+Lemma is_conflict_pattern_true {O} (pr : drules O) q :
+  conflict_pattern pr q <-> is_conflict_pattern pr q = true.
 Proof.
-  destruct drules_dec0.
-  unfold Decision. destruct q.
-  - right. intro. inv H.
-  - destruct q1, q2.
-    + right. intro. inv H.
-    + destruct q2_1. destruct q2_2.
-      * replace (IPatt HPatt o (IPatt HPatt o0 HPatt)) with (CR o o0); try reflexivity.
-        specialize dec_prio with (o1 := o) (o2 := o0).
-        specialize dec_left_a with (o1 := o) (o2 := o0).
-        destruct dec_prio, dec_left_a; auto using CPrio2, CLeft.
-        right. intro. inv H; contradiction.
-      * right. intro. inv H.
-      * right. intro. inv H.
-    + destruct q1_1. destruct q1_2.
-      * replace (IPatt (IPatt HPatt o0 HPatt) o HPatt) with (CL o o0); try reflexivity.
-        specialize dec_prio with (o1 := o) (o2 := o0).
-        specialize dec_right_a with (o1 := o) (o2 := o0).
-        destruct dec_prio, dec_right_a; auto using CPrio1, CRight.
-        right. intro. inv H; contradiction.
-      * right. intro. inv H.
-      * right. intro. inv H.
-    + right. intro. inv H.
+  split; intro.
+  - inv H; simpl; auto using decide_True, decide_False.
+    + destruct (decide (prio pr o1 o2)); auto using decide_True, decide_False.
+    + destruct (decide (prio pr o1 o2)); auto using decide_True, decide_False.
+  - destruct q; inv H.
+    destruct q1, q2; inv H1.
+    + destruct q2_1, q2_2; inv H0.
+      destruct (decide (prio pr o o0)); eauto with IGrammar.
+      destruct (decide (left_a pr o o0)); eauto with IGrammar.
+      inv H1.
+    + destruct q1_1, q1_2; inv H0.
+      destruct (decide (prio pr o o0)); eauto with IGrammar.
+      destruct (decide (right_a pr o o0)); eauto with IGrammar.
+      inv H1.
+    + destruct q1_1, q1_2; inv H0.
 Qed.
 
-Lemma linsert_one_exists {L O} (pr : drules O) `{drules_dec pr}
-    (l : L) (o : O) (t : parse_tree L O) :
-  exists t', linsert_one pr l o t t'.
+Lemma is_conflict_pattern_false {O} (pr : drules O) q :
+  ~ conflict_pattern pr q <-> is_conflict_pattern pr q = false.
+Proof.
+  split; intro.
+  - destruct (is_conflict_pattern pr q) eqn:E; auto.
+    exfalso. destruct H. apply is_conflict_pattern_true.
+    assumption.
+  - intro. apply is_conflict_pattern_true in H0.
+    rewrite H in H0. inv H0.
+Qed.
+
+(* This tactic can be used to rewrite to simplify a goal with a term
+   [linsert_one pr l1 o1 (INode t1 o2 t2))], creating two cases: one
+   where [CR o1 o2] is a conflict pattern and one where it is not a
+   conflict pattern. *)
+Ltac linsert_one_inode_destruct pr o1 o2 :=
+    cbn [linsert_one];
+     destruct (is_conflict_pattern pr (CR o1 o2)) eqn:E;
+     [apply is_conflict_pattern_true in E | apply is_conflict_pattern_false in E].
+
+(* Yield Preservation Lemmas *)
+
+Lemma linsert_one_yield_preserve {L O} (pr : drules O) (l1 : L) o1 t :
+  yield (linsert_one pr l1 o1 t) = inl l1 :: inr o1 :: yield t.
 Proof.
   induction t.
-  - eexists. apply ANode_LInsert_One.
-  - assert (Decision (conflict_pattern pr (CR o o0))). {
-      auto using dec_conflict_pattern.
-    }
-    destruct IHt1, IHt2.
-    destruct H.
-    + eexists. eauto using INode_LInsert_One_2.
-    + eexists. eauto using INode_LInsert_One_1.
-Qed.
-
-Lemma linsert_exists {L O} (pr : drules O) `{drules_dec pr}
-    (o : O) (t1 t2 : parse_tree L O) :
-  exists t', linsert pr t1 o t2 t'.
-Proof.
-  revert o t2. induction t1; intros.
-  - assert (exists t', linsert_one pr l o t2 t'). {
-      auto using linsert_one_exists.
-    }
-    destruct H. eauto using ANode_LInsert.
-  - specialize IHt1_2 with o0 t2. destruct IHt1_2.
-    specialize IHt1_1 with o x. destruct IHt1_1.
-    eauto using INode_LInsert.
-Qed.
-
-Lemma fix_tree_exists {L O} (pr : drules O) `{drules_dec pr} (t : parse_tree L O) :
-  exists t', fix_tree pr t t'.
-Proof.
-  induction t.
-  - eauto using ANode_fix.
-  - destruct IHt2 as [t2'].
-    assert (exists t', linsert pr t1 o t2' t'). {
-      auto using linsert_exists.
-    }
-    destruct H0 as [t'].
-    eauto using INode_fix.
-Qed.
-
-(* Yield Lemmas *)
-
-Lemma linsert_one_yield {L O} (pr : drules O)
-    (l1 : L) (o1 : O) (t t' : parse_tree L O) :
-  linsert_one pr l1 o1 t t' ->
-  yield t' = inl l1 :: inr o1 :: yield t .
-Proof.
-  intros. induction H; simpl; auto.
-  rewrite IHlinsert_one. reflexivity.
-Qed.
-
-Lemma linsert_yield {L O} (pr : drules O)
-    (o : O) (t1 t2 t' : parse_tree L O) :
-  linsert pr t1 o t2 t' ->
-  yield t' = yield t1 ++ inr o :: yield t2.
-Proof.
-  intro. induction H; simpl; eauto using linsert_one_yield.
-  - rewrite IHlinsert2. rewrite IHlinsert1.
-    simplify_list_eq. reflexivity.
-Qed.
-
-Lemma fix_tree_yield {L O} (pr : drules O) (t t' : parse_tree L O) :
-  fix_tree pr t t' ->
-  yield t' = yield t.
-Proof.
-  intro. induction H; simpl.
   - reflexivity.
-  - rewrite <- IHfix_tree.
-    apply linsert_yield in H0. rewrite H0.
+  - linsert_one_inode_destruct pr o1 o; simpl; auto.
+    rewrite IHt1. reflexivity.
+Qed.
+Hint Resolve linsert_one_yield_preserve : IGrammar.
+
+Lemma linsert_yield_preserve {L O} (pr : drules O) o (t1 t2 : parse_tree L O) :
+  yield (linsert pr t1 o t2) = yield t1 ++ inr o :: yield t2.
+Proof.
+  revert o t2.
+  induction t1; intros; simpl.
+  - auto with IGrammar.
+  - simplify_list_eq. rewrite <- IHt1_2. rewrite <- IHt1_1.
     reflexivity.
 Qed.
+Hint Resolve linsert_yield_preserve : IGrammar.
 
-(* Safe PR Lemmas *)
+(* Fixing a parse tree preserves its yield. *)
+Lemma fix_tree_yield_preserve {L O} (pr : drules O) (t : parse_tree L O) :
+  yield (fix_tree pr t) = yield t.
+Proof.
+  induction t; simpl.
+  - reflexivity.
+  - rewrite <- IHt2. auto with IGrammar.
+Qed.
 
-Lemma safe_cl_cr {O} (o1 o2 : O) (pr : drules O) `{safety_props pr} :
+(* For a safe disambiguation rules, it connot hold that both [CL o1 o2]
+   and [CR o2 o1] conflict patterns. *)
+Lemma safe_cl_cr {O} (o1 o2 : O) (pr : drules O) :
+  safe_pr pr ->
   (conflict_pattern pr (CL o1 o2) /\ conflict_pattern pr (CR o2 o1)) -> False.
 Proof.
-  intros H_CL_CR. destruct safety_props0.
-  destruct H_CL_CR as [H_CL H_CR].
-  inv H_CL; inv H_CR.
-  - apply prio_antisym in H0. contradiction.
-  - apply left_a_sym in H1.
-    apply prio_one in H0. destruct H0. contradiction.
-  - apply right_a_sym in H0.
-    apply prio_one in H1. destruct H1. contradiction.
-  - apply right_a_sym in H0.
-    apply left_a_one in H1. destruct H1. contradiction.
+  intros. destruct H0.
+  inv H0; inv H1; eapply H; eauto.
 Qed.
 
 (* Conflict-Free Lemmas *)
 
-Lemma linsert_one_match {L O} (pr : drules O) (l : L) (o1 : O) (t t' : parse_tree L O) :
-  linsert_one pr l o1 t t' ->
-  matches t' (IPatt HPatt o1 HPatt) \/
-  (exists o2 : O, matches t (IPatt HPatt o2 HPatt) /\ matches t' (IPatt HPatt o2 HPatt)).
+(* The top operator of [linsert_one l o t] either is [o] or remains the same as [t] *)
+Lemma linsert_one_top_operator_match {L O} (pr : drules O) (l : L) (o1 : O) (t : parse_tree L O) :
+  matches (linsert_one pr l o1 t) (IPatt HPatt o1 HPatt) \/
+  (exists o2, matches t (IPatt HPatt o2 HPatt) /\ matches (linsert_one pr l o1 t) (IPatt HPatt o2 HPatt)).
 Proof.
-  intros. inv H.
-  - left. apply IMatch; apply HMatch.
-  - left. apply IMatch; apply HMatch.
-  - right. exists o2. split; apply IMatch; apply HMatch.
+  destruct t.
+  - simpl. auto with IGrammar.
+  - linsert_one_inode_destruct pr o1 o; eauto 6 with IGrammar.
 Qed.
 
+(* Simple Lemma that states that proving something holds for all conflict patterns [q],
+   is the same as proving it holds for just conflict patterns of the form [CL] and [CR]. *)
 Lemma conflict_pattern_cases {O} (pr : drules O) (q : tree_pattern O) (P : Prop) :
   (forall o1 o2, q = CL o1 o2 -> P) ->
   (forall o1 o2, q = CR o1 o2 -> P) ->
@@ -154,67 +117,76 @@ Proof.
   intros. inv H1; eauto.
 Qed.
 
-Lemma linsert_one_safe {L O} (pr : drules O) `{safety_props pr}
-    (l1 : L) (o1 : O) (t t' : parse_tree L O) :
+(* This tactic applies the Lemma [conflict_pattern_cases] in a neat way. *)
+Ltac cp_cases H := eapply conflict_pattern_cases in H; try eassumption; intros; subst.
+
+(* A parse tree with just one infix node is always conflict-free *)
+Lemma inode_single_cfree {L O} (pr : drules O) (l1 l2 : L) (o : O) :
+  conflict_free (conflict_pattern pr) (INode (ANode l1) o (ANode l2)).
+Proof.
+  apply INode_cfree; auto using ANode_cfree.
+  intro. destruct H as [q]. inv H. cp_cases H0.
+  - inv H1. inv H3.
+  - inv H1. inv H8.
+Qed.
+
+(* Assuming the set of disambiguation rules is safe, one-left-inserting in a
+   conflict-free tree gives back also a conflict-free tree. *)
+Lemma linsert_one_safe {L O} (pr : drules O) (l1 : L) (o1 : O) (t : parse_tree L O) :
+  safe_pr pr ->
   conflict_free (conflict_pattern pr) t ->
-  linsert_one pr l1 o1 t t' ->
-  conflict_free (conflict_pattern pr) t'.
+  conflict_free (conflict_pattern pr) (linsert_one pr l1 o1 t).
 Proof.
-  intros. induction H0.
+  intros Hsafe Hcfree. induction t. apply inode_single_cfree.
+  linsert_one_inode_destruct pr o1 o.
+  - inv Hcfree. apply INode_cfree; auto. clear H3 H4.
+    intro. destruct H as [q]. inv H.
+    cp_cases H0.
+    + inv H1. inv H4. clear H9 H5 H7.
+      destruct (linsert_one_top_operator_match pr l1 o1 t1).
+      * rewrite <- H in H1. inv H1.
+        eauto using safe_cl_cr.
+      * rewrite <- H in H1.
+        inv H1. inv H3. inv H1. inv H4. clear H7 H9 H5 H12.
+        destruct H2. eexists. eauto with IGrammar.
+    + inv H1. inv H9. clear H4 H5 H7.
+      destruct H2. eexists. eauto with IGrammar.
   - apply INode_cfree; auto using ANode_cfree.
-    intro. inv H0. inv H1. inv H0; inv H2.
-    inv H4. inv H9. inv H9. inv H4.
-  - apply INode_cfree; auto using ANode_cfree.
-    intro. inv H1. inv H2. 
-    eapply conflict_pattern_cases; try eassumption; intros; subst; inv H3.
-    + inv H5.
-    + inv H10. eauto using safe_cl_cr.
-  - inv H. apply INode_cfree; auto.
-    intro. inv H. inv H2.
-    eapply conflict_pattern_cases; try eassumption; intros; subst; inv H3.
-    + apply linsert_one_match in H1. destruct H1.
-      * inv H1. inv H8. eauto using safe_cl_cr.
-      * inv H1. inv H2. inv H8. inv H3. inv H1.
-        apply H5. exists (CL o0 x). split; try assumption.
-        unfold CL. auto using HMatch, IMatch.
-    + inv H13. apply H5.
-      exists (CR o0 o3). split; try assumption.
-      unfold CR. auto using HMatch, IMatch.
+    intro. destruct H as [q]. inv H.
+    cp_cases H0.
+    + inv H1. inv H3.
+    + inv H1. inv H8. contradiction.
 Qed.
 
-Lemma linsert_safe {L O} (pr : drules O) `{safety_props pr}
-    (o : O) (t1 t2 t' : parse_tree L O) :
+Lemma linsert_safe {L O} (pr : drules O) (o : O) (t1 t2 : parse_tree L O) :
+  safe_pr pr ->
   conflict_free (conflict_pattern pr) t2 ->
-  linsert pr t1 o t2 t' ->
-  conflict_free (conflict_pattern pr) t'.
+  conflict_free (conflict_pattern pr) (linsert pr t1 o t2).
 Proof.
-  intros. induction H0; eauto using linsert_one_safe.
+  intro Hsafe. revert o t2.
+  induction t1; eauto using linsert_one_safe.
 Qed.
 
-Lemma fix_tree_safe {L O} (pr : drules O) `{safety_props pr} (t t' : parse_tree L O) :
-  fix_tree pr t t' ->
-  conflict_free (conflict_pattern pr) t'.
+Lemma fix_tree_safe {L O} (pr : drules O) (t t' : parse_tree L O) :
+  safe_pr pr ->
+  conflict_free (conflict_pattern pr) (fix_tree pr t).
 Proof.
-  intro. induction H.
+  intro. induction t.
   - apply ANode_cfree.
   - eauto using linsert_safe.
 Qed.
 
 (* Safety *)
 
-Theorem safety {L O} (pr : drules O) `{safety_props pr} `{drules_dec pr} (w : list (L + O)) :
+Theorem safety {L O} (pr : drules O) (w : list (L + O)) :
+  safe_pr pr ->
   language w -> dlanguage pr w.
 Proof.
+  intro Hsafe.
   unfold language, dlanguage. intro. destruct H as [t].
   rewrite <- H.
-  assert (exists t', fix_tree pr t t'). {
-    auto using fix_tree_exists.
-  }
-  destruct H0 as [t'].
-  exists t'.
-  split.
-  - eauto using fix_tree_yield.
-  - eauto using fix_tree_safe.
+  exists (fix_tree pr t).
+  eauto using fix_tree_yield_preserve, fix_tree_safe.
 Qed.
 
 End IGrammarSafety.
